progs/queue.v
@@ -7,23 +7,25 @@ Definition _next : ident := 7%positive.
 Definition ___builtin_annot_intval : ident := 3%positive.
 Definition ___builtin_fabs : ident := 1%positive.
 Definition _fifo_new : ident := 14%positive.
-Definition _make_elem : ident := 19%positive.
+Definition _n : ident := 19%positive.
 Definition _a : ident := 9%positive.
 Definition _mallocN : ident := 4%positive.
 Definition _fifo_put : ident := 17%positive.
 Definition _b : ident := 8%positive.
-Definition _fifo_get : ident := 18%positive.
+Definition _fifo_empty : ident := 18%positive.
 Definition _t : ident := 16%positive.
 Definition _Q : ident := 13%positive.
 Definition _struct_elem : ident := 6%positive.
 Definition _struct_fifo : ident := 12%positive.
+Definition _main : ident := 24%positive.
+Definition _j : ident := 23%positive.
 Definition _head : ident := 11%positive.
 Definition _freeN : ident := 5%positive.
 Definition ___builtin_memcpy_aligned : ident := 2%positive.
-Definition _j : ident := 21%positive.
+Definition _make_elem : ident := 21%positive.
 Definition _tail : ident := 10%positive.
-Definition _main : ident := 22%positive.
-Definition _i : ident := 20%positive.
+Definition _i : ident := 22%positive.
+Definition _fifo_get : ident := 20%positive.
 
 Definition t_struct_elem :=
    (Tstruct _struct_elem
@@ -49,16 +51,16 @@ Definition f_fifo_new := {|
   fn_return := (tptr t_struct_fifo);
   fn_params := nil;
   fn_vars := nil;
-  fn_temps := ((_Q, (tptr t_struct_fifo)) :: (23%positive, (tptr tvoid)) ::
+  fn_temps := ((_Q, (tptr t_struct_fifo)) :: (25%positive, (tptr tvoid)) ::
                nil);
   fn_body :=
 (Ssequence
   (Ssequence
-    (Scall (Some 23%positive)
+    (Scall (Some 25%positive)
       (Evar _mallocN (Tfunction (Tcons tint Tnil) (tptr tvoid)))
       ((Econst_int (Int.repr 8) tuint) :: nil))
     (Sset _Q
-      (Ecast (Etempvar 23%positive (tptr tvoid)) (tptr t_struct_fifo))))
+      (Ecast (Etempvar 25%positive (tptr tvoid)) (tptr t_struct_fifo))))
   (Ssequence
     (Sassign
       (Efield (Ederef (Etempvar _Q (tptr t_struct_fifo)) t_struct_fifo) _head
@@ -99,50 +101,75 @@ Definition f_fifo_put := {|
       (Sreturn None))))
 |}.
 
-Definition f_fifo_get := {|
-  fn_return := (tptr t_struct_elem);
+Definition f_fifo_empty := {|
+  fn_return := tint;
   fn_params := ((_Q, (tptr t_struct_fifo)) :: nil);
   fn_vars := nil;
-  fn_temps := ((_p, (tptr t_struct_elem)) ::
-               (_t, (tptr (tptr t_struct_elem))) :: nil);
+  fn_temps := ((_t, (tptr (tptr t_struct_elem))) :: nil);
   fn_body :=
 (Ssequence
   (Sset _t
     (Efield (Ederef (Etempvar _Q (tptr t_struct_fifo)) t_struct_fifo) _tail
       (tptr (tptr t_struct_elem))))
-  (Sifthenelse (Ebinop Oeq (Etempvar _t (tptr (tptr t_struct_elem)))
-                 (Eaddrof
-                   (Efield
-                     (Ederef (Etempvar _Q (tptr t_struct_fifo))
-                       t_struct_fifo) _head (tptr t_struct_elem))
-                   (tptr (tptr t_struct_elem))) tint)
-    (Sreturn (Some (Ecast (Econst_int (Int.repr 0) tint) (tptr tvoid))))
+  (Sreturn (Some (Ebinop Oeq (Etempvar _t (tptr (tptr t_struct_elem)))
+                   (Eaddrof
+                     (Efield
+                       (Ederef (Etempvar _Q (tptr t_struct_fifo))
+                         t_struct_fifo) _head (tptr t_struct_elem))
+                     (tptr (tptr t_struct_elem))) tint))))
+|}.
+
+Definition f_fifo_get := {|
+  fn_return := (tptr t_struct_elem);
+  fn_params := ((_Q, (tptr t_struct_fifo)) :: nil);
+  fn_vars := nil;
+  fn_temps := ((_p, (tptr t_struct_elem)) :: (_n, (tptr t_struct_elem)) ::
+               (_t, (tptr (tptr t_struct_elem))) :: nil);
+  fn_body :=
+(Ssequence
+  (Sset _p
+    (Efield (Ederef (Etempvar _Q (tptr t_struct_fifo)) t_struct_fifo) _head
+      (tptr t_struct_elem)))
+  (Ssequence
+    (Sset _t
+      (Efield (Ederef (Etempvar _Q (tptr t_struct_fifo)) t_struct_fifo) _tail
+        (tptr (tptr t_struct_elem))))
     (Ssequence
-      (Sset _p
-        (Efield (Ederef (Etempvar _Q (tptr t_struct_fifo)) t_struct_fifo)
-          _head (tptr t_struct_elem)))
-      (Ssequence
+      (Sifthenelse (Ebinop Oeq (Etempvar _t (tptr (tptr t_struct_elem)))
+                     (Eaddrof
+                       (Efield
+                         (Ederef (Etempvar _p (tptr t_struct_elem))
+                           t_struct_elem) _next (tptr t_struct_elem))
+                       (tptr (tptr t_struct_elem))) tint)
         (Sassign
           (Efield (Ederef (Etempvar _Q (tptr t_struct_fifo)) t_struct_fifo)
-            _head (tptr t_struct_elem))
-          (Efield (Ederef (Etempvar _p (tptr t_struct_elem)) t_struct_elem)
-            _next (tptr t_struct_elem)))
-        (Sreturn (Some (Etempvar _p (tptr t_struct_elem))))))))
+            _tail (tptr (tptr t_struct_elem)))
+          (Eaddrof
+            (Efield (Ederef (Etempvar _Q (tptr t_struct_fifo)) t_struct_fifo)
+              _head (tptr t_struct_elem)) (tptr (tptr t_struct_elem))))
+        (Ssequence
+          (Sset _n
+            (Efield (Ederef (Etempvar _p (tptr t_struct_elem)) t_struct_elem)
+              _next (tptr t_struct_elem)))
+          (Sassign
+            (Efield (Ederef (Etempvar _Q (tptr t_struct_fifo)) t_struct_fifo)
+              _head (tptr t_struct_elem)) (Etempvar _n (tptr t_struct_elem)))))
+      (Sreturn (Some (Etempvar _p (tptr t_struct_elem)))))))
 |}.
 
 Definition f_make_elem := {|
   fn_return := (tptr t_struct_elem);
   fn_params := ((_a, tint) :: (_b, tint) :: nil);
   fn_vars := nil;
-  fn_temps := ((_p, (tptr t_struct_elem)) :: (23%positive, (tptr tvoid)) ::
+  fn_temps := ((_p, (tptr t_struct_elem)) :: (25%positive, (tptr tvoid)) ::
                nil);
   fn_body :=
 (Ssequence
   (Ssequence
-    (Scall (Some 23%positive)
+    (Scall (Some 25%positive)
       (Evar _mallocN (Tfunction (Tcons tint Tnil) (tptr tvoid)))
       ((Econst_int (Int.repr 12) tuint) :: nil))
-    (Sset _p (Etempvar 23%positive (tptr tvoid))))
+    (Sset _p (Etempvar 25%positive (tptr tvoid))))
   (Ssequence
     (Sassign
       (Efield (Ederef (Etempvar _p (tptr t_struct_elem)) t_struct_elem) _a
@@ -160,24 +187,24 @@ Definition f_main := {|
   fn_vars := nil;
   fn_temps := ((_i, tint) :: (_j, tint) :: (_Q, (tptr t_struct_fifo)) ::
                (_p, (tptr t_struct_elem)) ::
+               (28%positive, (tptr t_struct_elem)) ::
+               (27%positive, (tptr t_struct_elem)) ::
                (26%positive, (tptr t_struct_elem)) ::
-               (25%positive, (tptr t_struct_elem)) ::
-               (24%positive, (tptr t_struct_elem)) ::
-               (23%positive, (tptr t_struct_fifo)) :: nil);
+               (25%positive, (tptr t_struct_fifo)) :: nil);
   fn_body :=
 (Ssequence
   (Ssequence
-    (Scall (Some 23%positive)
+    (Scall (Some 25%positive)
       (Evar _fifo_new (Tfunction Tnil (tptr t_struct_fifo))) nil)
-    (Sset _Q (Etempvar 23%positive (tptr t_struct_fifo))))
+    (Sset _Q (Etempvar 25%positive (tptr t_struct_fifo))))
   (Ssequence
     (Ssequence
-      (Scall (Some 24%positive)
+      (Scall (Some 26%positive)
         (Evar _make_elem (Tfunction (Tcons tint (Tcons tint Tnil))
                            (tptr t_struct_elem)))
         ((Econst_int (Int.repr 1) tint) :: (Econst_int (Int.repr 10) tint) ::
          nil))
-      (Sset _p (Etempvar 24%positive (tptr t_struct_elem))))
+      (Sset _p (Etempvar 26%positive (tptr t_struct_elem))))
     (Ssequence
       (Scall None
         (Evar _fifo_put (Tfunction
@@ -187,12 +214,12 @@ Definition f_main := {|
          (Etempvar _p (tptr t_struct_elem)) :: nil))
       (Ssequence
         (Ssequence
-          (Scall (Some 25%positive)
+          (Scall (Some 27%positive)
             (Evar _make_elem (Tfunction (Tcons tint (Tcons tint Tnil))
                                (tptr t_struct_elem)))
             ((Econst_int (Int.repr 2) tint) ::
              (Econst_int (Int.repr 20) tint) :: nil))
-          (Sset _p (Etempvar 25%positive (tptr t_struct_elem))))
+          (Sset _p (Etempvar 27%positive (tptr t_struct_elem))))
         (Ssequence
           (Scall None
             (Evar _fifo_put (Tfunction
@@ -202,11 +229,11 @@ Definition f_main := {|
              (Etempvar _p (tptr t_struct_elem)) :: nil))
           (Ssequence
             (Ssequence
-              (Scall (Some 26%positive)
+              (Scall (Some 28%positive)
                 (Evar _fifo_get (Tfunction (Tcons (tptr t_struct_fifo) Tnil)
                                   (tptr t_struct_elem)))
                 ((Etempvar _Q (tptr t_struct_fifo)) :: nil))
-              (Sset _p (Etempvar 26%positive (tptr t_struct_elem))))
+              (Sset _p (Etempvar 28%positive (tptr t_struct_elem))))
             (Ssequence
               (Sset _i
                 (Efield
@@ -256,6 +283,7 @@ prog_defs :=
      (Tcons (tptr tvoid) (Tcons tint Tnil)) tvoid)) ::
  (_fifo_new, Gfun(Internal f_fifo_new)) ::
  (_fifo_put, Gfun(Internal f_fifo_put)) ::
+ (_fifo_empty, Gfun(Internal f_fifo_empty)) ::
  (_fifo_get, Gfun(Internal f_fifo_get)) ::
  (_make_elem, Gfun(Internal f_make_elem)) ::
  (_main, Gfun(Internal f_main)) :: nil);
