progs/call_lemmas.v
@@ -1,0 +1,355 @@
+Load loadpath.
+Require Import Coqlib compositional_compcert.Coqlib2.
+Require Import veric.SeparationLogic.
+Require veric.SequentialClight.
+Import SequentialClight.SeqC.CSL.
+Require Import progs.client_lemmas.
+Require Import progs.field_mapsto.
+Require Import progs.assert_lemmas.
+
+Local Open Scope logic.
+
+Lemma semax_call': forall Delta A (Pre Post: A -> assert) (x: A) ret fsig a bl P Q R,
+   Cop.classify_fun (typeof a) = Cop.fun_case_f (type_of_params (fst fsig)) (snd fsig) ->
+   match fsig, ret with
+   | (_, Tvoid), None => True
+   | (_, Tvoid), Some _ => False
+   | _, Some _ => True
+   | _, _ => False
+   end ->
+  semax Delta
+         (PROPx P (LOCALx (tc_expr Delta a :: tc_exprlist Delta (snd (split (fst fsig))) bl :: Q)
+            (SEPx (`(Pre x) ( (make_args' fsig (eval_exprlist (snd (split (fst fsig))) bl))) ::
+                      `(fun_assert_emp fsig A Pre Post) (eval_expr a) :: R))))
+          (Scall ret a bl)
+          (normal_ret_assert 
+            (EX old:val, 
+              PROPx P (LOCALx (map (substopt ret (`old)) Q) 
+                (SEPx (`(Post x) (get_result ret) :: map (substopt ret (`old)) R))))).
+Proof.
+ intros.
+eapply semax_pre_post ; [ | | 
+   apply (semax_call Delta A Pre Post x (PROPx P (LOCALx Q (SEPx R))) ret fsig a bl H)].
+ Focus 3.
+ clear - H0.
+ destruct fsig. destruct t; destruct ret; simpl in *; try contradiction; split; intros; congruence.
+ intro rho; normalize.
+unfold fun_assert_emp.
+repeat rewrite corable_andp_sepcon2 by apply corable_fun_assert.
+normalize.
+rewrite corable_sepcon_andp1 by apply corable_fun_assert.
+rewrite sepcon_comm; auto. 
+intros.
+normalize.
+intro old.
+apply exp_right with old; destruct ret; normalize.
+intro rho; normalize.
+rewrite sepcon_comm; auto.
+intro rho; normalize.
+rewrite sepcon_comm; auto.
+unfold substopt.
+repeat rewrite list_map_identity.
+normalize.
+Qed.
+
+Lemma semax_call1: forall Delta A (Pre Post: A -> assert) (x: A) id fsig a bl P Q R,
+   Cop.classify_fun (typeof a) = Cop.fun_case_f (type_of_params (fst fsig)) (snd fsig) ->
+   match fsig with
+   | (_, Tvoid) => False
+   | _ => True
+   end ->
+  semax Delta
+         (PROPx P (LOCALx (tc_expr Delta a :: tc_exprlist Delta (snd (split (fst fsig))) bl :: Q)
+            (SEPx (`(Pre x) ( (make_args' fsig (eval_exprlist (snd (split (fst fsig))) bl))) ::
+                      `(fun_assert_emp fsig A Pre Post) (eval_expr a) :: R))))
+          (Scall (Some id) a bl)
+          (normal_ret_assert 
+            (EX old:val, 
+              PROPx P (LOCALx (map (subst id (`old)) Q) 
+                (SEPx (`(Post x) (get_result1 id) :: map (subst id (`old)) R))))).
+Proof.
+intros.
+apply semax_call'; auto.
+Qed.
+
+Lemma semax_call0: forall Delta A (Pre Post: A -> assert) (x: A) fsig a bl P Q R,
+   Cop.classify_fun (typeof a) = Cop.fun_case_f (type_of_params (fst fsig)) (snd fsig) ->
+   match fsig with
+   | (_, Tvoid) => True
+   | _ => False
+   end ->
+  semax Delta
+         (PROPx P (LOCALx (tc_expr Delta a :: tc_exprlist Delta (snd (split (fst fsig))) bl :: Q)
+            (SEPx (`(Pre x) ( (make_args' fsig (eval_exprlist (snd (split (fst fsig))) bl))) ::
+                      `(fun_assert_emp fsig A Pre Post) (eval_expr a) :: R))))
+          (Scall None a bl)
+          (normal_ret_assert 
+            (PROPx P (LOCALx Q (SEPx (`(Post x) (make_args nil nil) :: R))))).
+Proof.
+intros.
+eapply semax_pre_post ; [ | | 
+   apply (semax_call Delta A Pre Post x (PROPx P (LOCALx Q (SEPx R))) None fsig a bl H)].
+ Focus 3.
+ clear - H0.
+ destruct fsig. destruct t; simpl in *; try contradiction; split; intros; congruence.
+ intro rho; normalize.
+unfold fun_assert_emp.
+repeat rewrite corable_andp_sepcon2 by apply corable_fun_assert.
+normalize.
+rewrite corable_sepcon_andp1 by apply corable_fun_assert.
+rewrite sepcon_comm; auto. 
+intros.
+normalize.
+intro rho; normalize.
+rewrite sepcon_comm; auto.
+Qed.
+
+
+Lemma semax_fun_id':
+      forall id fsig (A : Type) (Pre Post : A -> assert)
+              Delta P Q R PostCond c
+            (GLBL: (var_types Delta) ! id = None),
+            (glob_types Delta) ! id = Some (Global_func (mk_funspec fsig A Pre Post)) ->
+       semax Delta 
+        (PROPx P (LOCALx Q (SEPx (`(fun_assert_emp fsig A Pre Post)
+                         (eval_lvalue (Evar id (type_of_funsig fsig))) :: R))))
+                              c PostCond ->
+       semax Delta (PROPx P (LOCALx Q (SEPx R))) c PostCond.
+Proof.
+intros. 
+apply (semax_fun_id id fsig A Pre Post Delta); auto.
+eapply semax_pre; [ | apply H0].
+forget (eval_lvalue (Evar id (type_of_funsig fsig))) as f.
+intro rho; normalize.
+rewrite andp_comm.
+unfold fun_assert_emp.
+rewrite corable_andp_sepcon2 by apply corable_fun_assert.
+rewrite emp_sepcon; auto.
+Qed.
+
+Lemma eqb_typelist_refl: forall tl, eqb_typelist tl tl = true.
+Proof.
+induction tl; simpl; auto.
+apply andb_true_iff.
+split; auto.
+apply eqb_type_refl.
+Qed.
+
+
+Lemma semax_call_id0:
+ forall Delta P Q R id argtys bl fsig A x Pre Post
+   (GLBL: (var_types Delta) ! id = None),
+   (glob_types Delta) ! id = Some (Global_func (mk_funspec fsig A Pre Post)) ->
+   match fsig with
+   | (_, Tvoid) => True
+   | _ => False
+   end ->
+   argtys = type_of_params (fst fsig) ->
+   Tvoid = snd fsig ->
+  semax Delta (PROPx P (LOCALx (tc_exprlist Delta (snd (split (fst fsig))) bl :: Q) (SEPx (`(Pre x) (make_args' fsig (eval_exprlist (snd (split (fst fsig))) bl)) :: R))))
+    (Scall None (Evar id (Tfunction argtys Tvoid)) bl)
+    (normal_ret_assert 
+       (PROPx P (LOCALx Q (SEPx (`(Post x) (make_args nil nil) :: R))))).
+Proof.
+intros.
+assert (Cop.classify_fun (typeof (Evar id (Tfunction argtys Tvoid)))=
+               Cop.fun_case_f (type_of_params (fst fsig)) (snd fsig)).
+rewrite <- H2; subst; reflexivity.
+apply semax_fun_id' with id fsig A Pre Post; auto.
+subst. 
+
+eapply semax_pre; [ | apply (semax_call0 Delta A Pre Post x fsig  _ bl P Q R H3 H0)].
+apply andp_left2.
+apply andp_derives; auto.
+apply andp_derives; auto.
+intro rho; simpl.
+subst.
+autorewrite with normalize.
+apply andp_right.
+apply prop_right. hnf.
+rewrite <- H2 in *.
+simpl.
+unfold get_var_type. rewrite GLBL. rewrite H.
+simpl.
+rewrite eqb_typelist_refl.
+simpl. rewrite <- H2. split; hnf; auto.
+auto.
+change SEPx with SEPx'.
+simpl.
+intro rho.
+rewrite H2.
+rewrite sepcon_comm.
+rewrite sepcon_assoc.
+autorewrite with normalize.
+apply sepcon_derives; auto.
+rewrite sepcon_comm.
+apply sepcon_derives; auto.
+Qed.
+
+Lemma semax_call_id1:
+ forall Delta P Q R ret id argtys retty bl fsig A x Pre Post
+   (GLBL: (var_types Delta) ! id = None),
+   (glob_types Delta) ! id = Some (Global_func (mk_funspec fsig A Pre Post)) ->
+   match fsig with
+   | (_, Tvoid) => False
+   | _ => True
+   end ->
+   argtys = type_of_params (fst fsig) ->
+   retty = snd fsig ->
+  semax Delta (PROPx P (LOCALx (tc_exprlist Delta (snd (split (fst fsig))) bl :: Q) (SEPx (`(Pre x) (make_args' fsig (eval_exprlist (snd (split (fst fsig))) bl)) :: R))))
+    (Scall (Some ret)
+             (Evar id (Tfunction argtys retty))
+             bl)
+    (normal_ret_assert 
+       (EX old:val, 
+          PROPx P (LOCALx (map (subst ret (`old)) Q) 
+             (SEPx (`(Post x) (get_result1 ret) :: map (subst ret (`old)) R))))).
+Proof.
+intros.
+assert (Cop.classify_fun (typeof (Evar id (Tfunction argtys retty)))=
+               Cop.fun_case_f (type_of_params (fst fsig)) (snd fsig)).
+subst; reflexivity.
+apply semax_fun_id' with id fsig A Pre Post; auto.
+subst. 
+eapply semax_pre; [ | apply (semax_call1 Delta A Pre Post x ret fsig  _ bl P Q R H3 H0)].
+apply andp_left2.
+apply andp_derives; auto.
+apply andp_derives; auto.
+intro rho; simpl.
+subst.
+autorewrite with normalize.
+apply andp_right.
+apply prop_right. hnf.
+simpl.
+unfold get_var_type. rewrite GLBL. rewrite H.
+simpl.
+rewrite eqb_typelist_refl.
+rewrite eqb_type_refl.
+simpl. split; hnf; auto.
+auto.
+change SEPx with SEPx'.
+simpl.
+intro rho.
+rewrite sepcon_comm.
+rewrite sepcon_assoc.
+autorewrite with normalize.
+apply sepcon_derives; auto.
+rewrite sepcon_comm.
+apply sepcon_derives; auto.
+Qed.
+
+
+Lemma semax_call_id1':
+ forall Delta P Q R ret id argtys retty bl fsig A x Pre Post
+   (GLBL: (var_types Delta) ! id = None),
+   (glob_types Delta) ! id = Some (Global_func (mk_funspec fsig A Pre Post)) ->
+   match fsig with
+   | (_, Tvoid) => False
+   | _ => True
+   end ->
+   argtys = type_of_params (fst fsig) ->
+   retty = snd fsig ->
+  forall 
+   (CLOSQ: Forall (closed_wrt_vars (eq ret)) Q)
+   (CLOSR: Forall (closed_wrt_vars (eq ret)) R),
+  semax Delta (PROPx P (LOCALx (tc_exprlist Delta (snd (split (fst fsig))) bl :: Q) (SEPx (`(Pre x) (make_args' fsig (eval_exprlist (snd (split (fst fsig))) bl)) :: R))))
+    (Scall (Some ret)
+             (Evar id (Tfunction argtys retty))
+             bl)
+    (normal_ret_assert 
+       (PROPx P (LOCALx Q   (SEPx (`(Post x) (get_result1 ret) ::  R))))).
+Proof.
+intros.
+eapply semax_post;
+  [ | apply (semax_call_id1 Delta P Q R ret id argtys retty bl fsig A x Pre Post 
+     GLBL H H0 H1 H2)].
+intros ek vl.
+apply andp_left2.
+unfold normal_ret_assert.
+apply andp_derives; auto.
+apply andp_derives; auto.
+apply exp_left; intro v.
+apply andp_derives; auto.
+apply andp_derives.
+unfold local, lift1 ;intro rho.
+clear - CLOSQ.
+apply prop_left. intro.
+apply prop_right.
+induction Q; simpl; auto.
+inv CLOSQ.
+destruct H.
+split.
+rewrite closed_wrt_subst in H; auto.
+auto.
+clear - CLOSR.
+change SEPx with SEPx'.
+unfold SEPx'. intro rho.
+simpl.
+apply sepcon_derives; auto.
+induction R; simpl; auto.
+inv CLOSR.
+apply sepcon_derives.
+rewrite closed_wrt_subst; auto.
+apply IHR; auto.
+Qed.
+
+Lemma semax_call_id1_Eaddrof:
+ forall Delta P Q R ret id argtys retty bl fsig A x Pre Post
+   (GLBL: (var_types Delta) ! id = None),
+   (glob_types Delta) ! id = Some (Global_func (mk_funspec fsig A Pre Post)) ->
+   match fsig with
+   | (_, Tvoid) => False
+   | _ => True
+   end ->
+   argtys = type_of_params (fst fsig) ->
+   retty = snd fsig ->
+  semax Delta (PROPx P (LOCALx (tc_exprlist Delta (snd (split (fst fsig))) bl :: Q) (SEPx (`(Pre x) (make_args' fsig (eval_exprlist (snd (split (fst fsig))) bl)) :: R))))
+    (Scall (Some ret)
+             (Eaddrof (Evar id (Tfunction argtys retty)) (Tpointer (Tfunction argtys retty) noattr))
+             bl)
+    (normal_ret_assert 
+       (EX old:val, 
+          PROPx P (LOCALx (map (subst ret (`old)) Q) 
+             (SEPx (`(Post x) (get_result1 ret) :: map (subst ret (`old)) R))))).
+Proof.
+intros.
+assert (Cop.classify_fun (typeof (Eaddrof (Evar id (Tfunction argtys retty)) (Tpointer (Tfunction argtys retty) noattr)))=
+               Cop.fun_case_f (type_of_params (fst fsig)) (snd fsig)).
+subst; reflexivity.
+apply semax_fun_id' with id fsig A Pre Post; auto.
+subst. 
+eapply semax_pre; [ | apply (semax_call1 Delta A Pre Post x ret fsig  _ bl P Q R H3 H0)].
+apply andp_left2.
+apply andp_derives; auto.
+apply andp_derives; auto.
+intro rho; simpl.
+subst.
+autorewrite with normalize.
+apply andp_right.
+apply prop_right. hnf.
+simpl.
+unfold get_var_type. rewrite GLBL. rewrite H.
+simpl.
+rewrite eqb_typelist_refl.
+rewrite eqb_type_refl.
+simpl. apply I.
+auto.
+change SEPx with SEPx'.
+simpl.
+intro rho.
+cancel.
+Qed.
+
+
+Lemma semax_call_id_aux1: forall P Q1 Q R S,
+     PROPx P (LOCALx (Q1::Q) R) |-- S -> local Q1 && PROPx P (LOCALx Q R) |-- S.
+Proof. intros. eapply derives_trans; try apply H.
+  intro rho; normalize.
+ unfold PROPx. simpl.
+ apply andp_derives; auto.
+ unfold LOCALx. simpl.
+ unfold local,lift2,lift1.
+ apply derives_extract_prop; intro.
+ apply andp_right; auto.
+ apply prop_right; split; auto.
+Qed.
