progs/forward.v
@@ -6,9 +6,167 @@ Import SequentialClight.SeqC.CSL.
 Require Import progs.client_lemmas.
 Require Import progs.field_mapsto.
 Require Import progs.assert_lemmas.
-Require Export progs.forward_lemmas.
+Require Export progs.forward_lemmas progs.call_lemmas.
 
 Local Open Scope logic.
+
+(* BEGIN HORRIBLE1.
+  The following lemma is needed because CompCert clightgen
+ produces the following AST for function call:
+  (Ssequence (Scall (Some id') ... ) (Sset id (Etempvar id' _)))
+instead of the more natural
+   (Scall id ...)
+Our general tactics are powerful enough to reason about the sequence,
+one statement at a time, but it is not nice to burden the user with knowing
+about id'.  So we handle it all in one gulp.
+ See also BEGIN HORRIBLE1 in forward.v
+*)
+
+
+Lemma semax_call_id1_x:
+ forall Delta P Q R ret ret' id argtys retty bl fsig A x Pre Post
+   (GLBL: (var_types Delta) ! id = None),
+   (glob_types Delta) ! id = Some (Global_func (mk_funspec fsig A Pre Post)) ->
+   match fsig with
+   | (_, Tvoid) => False
+   | _ => True
+   end ->
+   argtys = type_of_params (fst fsig) ->
+   retty = snd fsig ->
+  forall
+   (CLOSQ: Forall (closed_wrt_vars (eq ret')) Q)
+   (CLOSR: Forall (closed_wrt_vars (eq ret')) R),
+   type_is_volatile retty = false -> 
+   (temp_types Delta) ! ret' = Some (retty, false) ->
+   is_neutral_cast retty retty = true ->
+   match (temp_types Delta) ! ret with Some (t,_) => eqb_type t retty | None => false end = true ->
+  semax Delta (PROPx P (LOCALx (tc_exprlist Delta (snd (split (fst fsig))) bl :: Q) (SEPx (`(Pre x) (make_args' fsig (eval_exprlist (snd (split (fst fsig))) bl)) :: R))))
+    (Ssequence (Scall (Some ret')
+             (Evar id (Tfunction argtys retty))
+             bl)
+      (Sset ret (Etempvar ret' retty)))
+    (normal_ret_assert 
+       (EX old:val, 
+          PROPx P (LOCALx (map (subst ret (`old)) Q) 
+             (SEPx (`(Post x) (get_result1 ret) :: map (subst ret (`old)) R))))).
+Proof.
+ intros. rename H3 into NONVOL.
+ eapply semax_seq'.
+ apply (semax_call_id1' _ P Q R ret' _ _ _ bl _ _ x _ _ GLBL H H0 H1 H2 CLOSQ CLOSR).
+match goal with |- semax ?D (PROPx ?P ?QR) ?c ?Post =>
+   assert ( (fold_right and True P) -> semax D (PROPx nil QR) c Post)
+ end.
+Focus 2.
+ clear - H3.
+ unfold PROPx. 
+ unfold PROPx at 1 in H3.
+ normalize in H3.
+ apply semax_extract_prop. apply H3.
+ (* End Focus 2 *)
+ intro.
+ apply semax_post_flipped
+ with (normal_ret_assert (EX  x0 : val,
+PROP  ()
+(LOCALx
+   (tc_environ
+      (initialized ret
+         (update_tycon Delta
+            (Scall (Some ret') (Evar id (Tfunction argtys retty)) bl)))
+    :: `eq (eval_id ret)
+         (subst ret (`x0) (eval_expr (Etempvar ret' retty)))
+       :: map (subst ret (`x0)) Q)
+   (SEPx
+      (map (subst ret (`x0)) (`(Post x) (get_result1 ret') :: R)))))).
+  make_sequential;
+          eapply semax_post_flipped;
+          [ apply forward_setx; 
+            try solve [intro rho; rewrite andp_unfold; apply andp_right; apply prop_right;
+                            repeat split ]
+           | intros ?ek ?vl; apply after_set_special1 ].
+ apply andp_right.
+ intro rho; unfold tc_expr; simpl.
+ rewrite NONVOL. simpl.
+ replace ( (temp_types (initialized ret' Delta)) ! ret' ) 
+     with (Some (retty, true)).
+Focus 2.
+ unfold initialized;  simpl. rewrite H4.
+ unfold temp_types; simpl.
+ rewrite PTree.gss. auto.
+ (* End Focus 2 *)
+ unfold local; apply prop_right.
+ simpl. rewrite eqb_type_refl. apply I.
+ intro rho; apply prop_right; unfold tc_temp_id; simpl.
+ unfold typecheck_temp_id.
+ destruct (eq_dec ret' ret).
+ subst ret'.
+ unfold temp_types. unfold initialized; simpl.
+ rewrite H4. simpl. rewrite PTree.gss.
+ rewrite H5.
+ simpl.
+ unfold isCastResultType. unfold is_neutral_cast in H5.
+ destruct (Cop.classify_cast retty retty); try discriminate.
+ rewrite eqb_type_refl. apply I.
+ unfold temp_types. unfold initialized; simpl.
+ rewrite H4. simpl. rewrite PTree.gso by auto. 
+ destruct ((temp_types Delta) ! ret); try discriminate.
+ destruct p. apply eqb_type_true in H6.
+ subst t. rewrite H5.
+ simpl.
+ unfold isCastResultType. unfold is_neutral_cast in H5.
+ destruct (Cop.classify_cast retty retty); try discriminate.
+ rewrite eqb_type_refl. apply I.
+ auto.
+ intros.
+ apply andp_left2. apply normal_ret_assert_derives'.
+ apply exp_derives; intro old.
+ apply andp_derives.
+ apply prop_right; auto.
+ intro rho; unfold LOCALx, local.
+change SEPx with SEPx'.
+ simpl. 
+  normalize.
+ unfold coerce, lift1_C, lift0_C.
+ apply sepcon_derives; auto.
+ normalize.
+ replace (subst ret (lift0 old) (get_result1 ret') rho)
+   with (get_result1 ret rho); auto.
+ destruct (eq_dec ret ret').
+ subst.
+ unfold get_result1.
+ unfold subst. f_equal.
+ normalize in H8.
+ normalize. f_equal. auto.
+ clear - H6 H8 H7.
+ unfold tc_environ in H7.
+ unfold env_set. destruct rho; simpl in *; f_equal.
+ unfold eval_id in H8; simpl in H8. unfold subst in H8.
+ simpl in *. rewrite Map.gss in H8. simpl in H8.
+ unfold_coerce. subst.
+ unfold Map.set. extensionality i. 
+ destruct (ident_eq i ret'); auto.  subst i.
+ unfold typecheck_environ in H7.
+ repeat rewrite andb_true_iff in H7.
+ destruct H7 as [[[? _] _] _].
+ simpl te_of in H.
+ apply environ_lemmas.typecheck_te_eqv in H.
+ hnf in H.
+ specialize (H ret').
+ revert H6; case_eq ((temp_types Delta)!ret'); intros; try discriminate.
+ destruct p.
+ unfold temp_types, initialized in H; simpl in H.
+ rewrite H0 in H. unfold temp_types in *. simpl in H. rewrite PTree.gss in H.
+ simpl in H. rewrite PTree.gss in H.
+ specialize (H true t (eq_refl _)). 
+ destruct H as [v [? ?]]. rewrite H.
+ apply H.
+  rewrite closed_wrt_subst; auto with closed.
+ unfold get_result1.
+ f_equal. f_equal.
+ rewrite H8.
+  rewrite closed_wrt_subst; auto with closed.
+Qed.
+
+(* END HORRIBLE1 *)
 
 Ltac normalizex :=
   normalize;
@@ -84,39 +242,6 @@ match goal with |- semax ?Delta (PROPx ?P (LOCALx ?Q (SEPx ?R)))
      ]
 end.
 
-Lemma field_mapsto_storable_at1:
-  forall Delta P Q sh ty fld e v R c Post,
-    semax Delta (PROPx P (LOCALx Q (SEPx (`(field_storable sh ty fld) e :: R)))) c Post ->
-    semax Delta (PROPx P (LOCALx Q (SEPx (`(field_mapsto sh ty fld) e v :: R)))) c Post.
-Proof.
-intros.
- eapply semax_pre0; [ | apply H].
- change SEPx with SEPx'.
- intro rho; unfold PROPx, LOCALx, SEPx'.
- simpl.
- apply andp_derives; auto.
- apply andp_derives; auto.
- apply sepcon_derives; auto.
- apply field_mapsto_storable.
-Qed.
-
-Lemma later_field_mapsto_storable_at1:
-  forall Delta P Q sh ty fld e v R c Post,
-    semax Delta (PROPx P (LOCALx Q (SEPx (|>`(field_storable sh ty fld) e :: R)))) c Post ->
-    semax Delta (PROPx P (LOCALx Q (SEPx (|> `(field_mapsto sh ty fld) e v :: R)))) c Post.
-Proof.
-intros.
- eapply semax_pre0; [ | apply H].
- change SEPx with SEPx'.
- intro rho; unfold PROPx, LOCALx, SEPx'.
- simpl.
- apply andp_derives; auto.
- apply andp_derives; auto.
- apply sepcon_derives; auto.
- apply later_derives; auto.
- apply field_mapsto_storable.
-Qed.
-
 
 Ltac isolate_mapsto_tac e R := 
   match R with 
@@ -129,59 +254,6 @@ Ltac isolate_mapsto_tac e R :=
              in rewrite (grab_nth_SEP (n- S n')); simpl minus; unfold nth, delete_nth; normalize;
                 replace e' with (eval_expr e) by auto
      end.
-
-Lemma mapsto_isptr:
-  forall sh t v1 v2,
-   mapsto sh t v1 v2 = !! (denote_tc_isptr v1) && mapsto sh t v1 v2.
-Proof.
-intros; unfold mapsto.
-destruct (access_mode t); normalize.
-destruct v1; normalize.
-Qed.
-
-Lemma semax_store_PQR:
-forall (Delta: tycontext) sh t1 P Q R e1 e2 x
-    (WS: writable_share sh)
-    (NONVOL: type_is_volatile t1 = false)
-    (TC: typecheck_store (Ederef e1 t1)),
-    typeof e1 = Tpointer t1 noattr ->
-    semax Delta 
-       (|> PROPx P (LOCALx (tc_expr Delta e1::tc_expr Delta (Ecast e2 t1)::Q)
-                             (SEPx (`(mapsto sh t1) (eval_expr e1) x::R))))
-       (Sassign (Ederef e1 t1) e2) 
-       (normal_ret_assert
-          (PROPx P (LOCALx Q
-              (SEPx  (`(mapsto sh t1) (eval_expr e1) 
-                  (`(eval_cast (typeof e2) t1) (eval_expr e2)) :: R))))).
-Proof.
-intros.
-pose proof semax_store.
-unfold coerce, lift2_C, lift1_C in *.
-eapply semax_pre_post; [ | | eapply H0]; try eassumption.
-instantiate (1:=(PROPx P (LOCALx Q (SEPx R)))).
-instantiate (1:= x (*lift1 (eval_cast (typeof e2) (typeof e1)) (eval_expr e2) *)).
-apply andp_left2. apply later_derives. change SEPx with SEPx'.
-intro rho; unfold PROPx, LOCALx, SEPx', local, lift1,lift2.
-simpl.
-normalize.
-unfold tc_lvalue. simpl typecheck_lvalue.
-rewrite H; simpl.
-rewrite mapsto_isptr at 1. normalize.
-repeat apply andp_right; try apply prop_right; auto.
-repeat rewrite denote_tc_assert_andp.
-repeat split; auto.
-rewrite NONVOL; hnf; auto.
-replace (force_ptr (eval_expr e1 rho)) with (eval_expr e1 rho); auto.
-clear - H5; hnf in H5. destruct (eval_expr e1 rho); try contradiction; simpl; auto.
-
-intros ek vl rho; unfold normal_ret_assert, local; unfold_coerce; simpl.
-normalize.
-cancel.
-clear.
-rewrite mapsto_isptr at 1. normalize.
-replace (force_ptr (eval_expr e1 rho)) with (eval_expr e1 rho); auto.
-destruct (eval_expr e1 rho); simpl in *; try contradiction; auto.
-Qed.
 
 Ltac isolate_storable_tac e fld R := 
   match R with 
@@ -218,7 +290,7 @@ Ltac store_field_tac :=
                 (SEPx R))));
    [ try solve [go_lower; normalize]
    | isolate_storable_tac e fld R; hoist_later_in_pre;
-       eapply semax_post'; [ | store_field_tac1]
+       eapply semax_post''; [ | store_field_tac1]
    ]
   end.
 
@@ -231,7 +303,7 @@ Ltac store_tac :=
                 (SEPx R))));
    [ try solve [go_lower; normalize]
    |  isolate_mapsto_tac e R; hoist_later_in_pre;
-       eapply semax_post';  
+       eapply semax_post'';  
        [ | eapply semax_store_PQR; [ auto | reflexivity | hnf; intuition | reflexivity ]
        ]
    ]
@@ -390,6 +462,11 @@ Ltac redefine_Delta :=
        match goal with |- semax (?D: tycontext) _ _ _ => 
            set (Delta:=D); change tycontext in (type of Delta)
        end
+  | Delta:= _: tycontext |- semax (join_tycon _ _) _ _ _ =>
+       unfold Delta in *; clear Delta;
+       match goal with |- semax (?D: tycontext) _ _ _ => 
+           set (Delta:=D); change tycontext in (type of Delta)
+       end
   | |- _ => idtac
 end.
 
@@ -408,6 +485,11 @@ Ltac forward1 :=
   | |- semax _ _ (Sassign (Ederef _ _) _) _ =>      store_tac
   | |- semax _ _ (Sset _ (Efield _ _ _)) _ => semax_field_tac || fail 2
   | |- semax _ _ (Sset ?id ?e) _ => forward_setx
+  | |- semax ?Delta (PROPx ?P (LOCALx ?Q ?R)) 
+                                 (Sifthenelse ?e _ _) _ =>
+            apply semax_pre_PQR
+                     with (PROPx P (LOCALx (tc_expr Delta e :: Q) R));
+             [ | apply semax_ifthenelse_PQR; [ reflexivity | | ]]
   | |- semax _ _ (Sreturn _) _ => 
                     eapply semax_pre; [ go_lower1 | apply semax_return ]
 (* see comment HACK below, in forward tactic...
