progs/forward_lemmas.v
@@ -369,16 +369,37 @@ intros x ?; apply exp_right with x.
 normalize.
 Qed.
 
-Lemma field_storable_nonnull:  forall t fld sh x, 
-     field_storable sh t fld x = 
-               !! (Cop.bool_val x (Tpointer t noattr) = Some true) && field_storable sh t fld x.
+Lemma field_mapsto_storable_at1:
+  forall Delta P Q sh ty fld e v R c Post,
+    semax Delta (PROPx P (LOCALx Q (SEPx (`(field_storable sh ty fld) e :: R)))) c Post ->
+    semax Delta (PROPx P (LOCALx Q (SEPx (`(field_mapsto sh ty fld) e v :: R)))) c Post.
 Proof.
 intros.
-apply pred_ext; normalize.
-apply andp_right; auto.
-unfold field_storable.
-unfold Cop.bool_val.
-destruct x; normalize.
+ eapply semax_pre0; [ | apply H].
+ change SEPx with SEPx'.
+ intro rho; unfold PROPx, LOCALx, SEPx'.
+ simpl.
+ apply andp_derives; auto.
+ apply andp_derives; auto.
+ apply sepcon_derives; auto.
+ apply field_mapsto_storable.
+Qed.
+
+Lemma later_field_mapsto_storable_at1:
+  forall Delta P Q sh ty fld e v R c Post,
+    semax Delta (PROPx P (LOCALx Q (SEPx (|>`(field_storable sh ty fld) e :: R)))) c Post ->
+    semax Delta (PROPx P (LOCALx Q (SEPx (|> `(field_mapsto sh ty fld) e v :: R)))) c Post.
+Proof.
+intros.
+ eapply semax_pre0; [ | apply H].
+ change SEPx with SEPx'.
+ intro rho; unfold PROPx, LOCALx, SEPx'.
+ simpl.
+ apply andp_derives; auto.
+ apply andp_derives; auto.
+ apply sepcon_derives; auto.
+ apply later_derives; auto.
+ apply field_mapsto_storable.
 Qed.
 
 Lemma semax_store_field':
@@ -421,6 +442,51 @@ simpl typeof. simpl force_ptr. auto.
 intros ek vl rho; unfold normal_ret_assert, local; unfold_coerce; simpl.
 normalize.
 Qed.
+
+Lemma semax_store_PQR:
+forall (Delta: tycontext) sh t1 P Q R e1 e2 x
+    (WS: writable_share sh)
+    (NONVOL: type_is_volatile t1 = false)
+    (TC: typecheck_store (Ederef e1 t1)),
+    typeof e1 = Tpointer t1 noattr ->
+    semax Delta 
+       (|> PROPx P (LOCALx (tc_expr Delta e1::tc_expr Delta (Ecast e2 t1)::Q)
+                             (SEPx (`(mapsto sh t1) (eval_expr e1) x::R))))
+       (Sassign (Ederef e1 t1) e2) 
+       (normal_ret_assert
+          (PROPx P (LOCALx Q
+              (SEPx  (`(mapsto sh t1) (eval_expr e1) 
+                  (`(eval_cast (typeof e2) t1) (eval_expr e2)) :: R))))).
+Proof.
+intros.
+pose proof semax_store.
+unfold coerce, lift2_C, lift1_C in *.
+eapply semax_pre_post; [ | | eapply H0]; try eassumption.
+instantiate (1:=(PROPx P (LOCALx Q (SEPx R)))).
+instantiate (1:= x (*lift1 (eval_cast (typeof e2) (typeof e1)) (eval_expr e2) *)).
+apply andp_left2. apply later_derives. change SEPx with SEPx'.
+intro rho; unfold PROPx, LOCALx, SEPx', local, lift1,lift2.
+simpl.
+normalize.
+unfold tc_lvalue. simpl typecheck_lvalue.
+rewrite H; simpl.
+rewrite mapsto_isptr at 1. normalize.
+repeat apply andp_right; try apply prop_right; auto.
+repeat rewrite denote_tc_assert_andp.
+repeat split; auto.
+rewrite NONVOL; hnf; auto.
+replace (force_ptr (eval_expr e1 rho)) with (eval_expr e1 rho); auto.
+clear - H5; hnf in H5. destruct (eval_expr e1 rho); try contradiction; simpl; auto.
+
+intros ek vl rho; unfold normal_ret_assert, local; unfold_coerce; simpl.
+normalize.
+cancel.
+clear.
+rewrite mapsto_isptr at 1. normalize.
+replace (force_ptr (eval_expr e1 rho)) with (eval_expr e1 rho); auto.
+destruct (eval_expr e1 rho); simpl in *; try contradiction; auto.
+Qed.
+
 
 Lemma forward_setx':
   forall Delta P id e,
@@ -520,15 +586,6 @@ Proof.
  apply prop_derives; intros [? ?]; auto.
 Qed.
 
-Lemma semax_post_flipped:
-  forall (R' : ret_assert) (Delta : tycontext) (R : ret_assert)
-         (P : assert) (c : statement),
-        semax Delta P c R' -> 
-       (forall (ek : exitkind) (vl : option val),
-        local (tc_environ (exit_tycon c Delta ek)) && R' ek vl |-- R ek vl) ->
-       semax Delta P c R.
-Proof. intros; eapply semax_post; eassumption. Qed.
-
 Lemma semax_load_assist1:
   forall B P Q1 Q R,
   (forall rho, Q1 rho = True) ->
@@ -546,506 +603,22 @@ Proof.
 destruct (split l); f_equal; auto.
 Qed.
 
-Lemma semax_call': forall Delta A (Pre Post: A -> assert) (x: A) ret fsig a bl P Q R,
-   Cop.classify_fun (typeof a) = Cop.fun_case_f (type_of_params (fst fsig)) (snd fsig) ->
-   match fsig, ret with
-   | (_, Tvoid), None => True
-   | (_, Tvoid), Some _ => False
-   | _, Some _ => True
-   | _, _ => False
-   end ->
-  semax Delta
-         (PROPx P (LOCALx (tc_expr Delta a :: tc_exprlist Delta (snd (split (fst fsig))) bl :: Q)
-            (SEPx (`(Pre x) ( (make_args' fsig (eval_exprlist (snd (split (fst fsig))) bl))) ::
-                      `(fun_assert_emp fsig A Pre Post) (eval_expr a) :: R))))
-          (Scall ret a bl)
-          (normal_ret_assert 
-            (EX old:val, 
-              PROPx P (LOCALx (map (substopt ret (`old)) Q) 
-                (SEPx (`(Post x) (get_result ret) :: map (substopt ret (`old)) R))))).
+Lemma semax_ifthenelse_PQR : 
+   forall Delta P Q R (b: expr) c d Post,
+      bool_type (typeof b) = true ->
+     semax Delta (PROPx P (LOCALx (`(typed_true (typeof b)) (eval_expr b) :: Q) (SEPx R)))
+                        c Post -> 
+     semax Delta (PROPx P (LOCALx (`(typed_false (typeof b)) (eval_expr b) :: Q) (SEPx R)))
+                        d Post -> 
+     semax Delta (PROPx P (LOCALx (tc_expr Delta b :: Q) (SEPx R)))
+                         (Sifthenelse b c d) Post.
 Proof.
  intros.
-eapply semax_pre_post ; [ | | 
-   apply (semax_call Delta A Pre Post x (PROPx P (LOCALx Q (SEPx R))) ret fsig a bl H)].
- Focus 3.
- clear - H0.
- destruct fsig. destruct t; destruct ret; simpl in *; try contradiction; split; intros; congruence.
- intro rho; normalize.
-unfold fun_assert_emp.
-repeat rewrite corable_andp_sepcon2 by apply corable_fun_assert.
-normalize.
-rewrite corable_sepcon_andp1 by apply corable_fun_assert.
-rewrite sepcon_comm; auto. 
-intros.
-normalize.
-intro old.
-apply exp_right with old; destruct ret; normalize.
-intro rho; normalize.
-rewrite sepcon_comm; auto.
-intro rho; normalize.
-rewrite sepcon_comm; auto.
-unfold substopt.
-repeat rewrite list_map_identity.
-normalize.
+ eapply semax_pre0; [ | apply semax_ifthenelse]; auto.
+ instantiate (1:=(PROPx P (LOCALx Q (SEPx R)))).
+ unfold PROPx, LOCALx; intro rho; normalize.
+ eapply semax_pre0; [ | eassumption].
+ unfold PROPx, LOCALx; intro rho; normalize.
+ eapply semax_pre0; [ | eassumption].
+ unfold PROPx, LOCALx; intro rho; normalize.
 Qed.
-
-Lemma semax_call1: forall Delta A (Pre Post: A -> assert) (x: A) id fsig a bl P Q R,
-   Cop.classify_fun (typeof a) = Cop.fun_case_f (type_of_params (fst fsig)) (snd fsig) ->
-   match fsig with
-   | (_, Tvoid) => False
-   | _ => True
-   end ->
-  semax Delta
-         (PROPx P (LOCALx (tc_expr Delta a :: tc_exprlist Delta (snd (split (fst fsig))) bl :: Q)
-            (SEPx (`(Pre x) ( (make_args' fsig (eval_exprlist (snd (split (fst fsig))) bl))) ::
-                      `(fun_assert_emp fsig A Pre Post) (eval_expr a) :: R))))
-          (Scall (Some id) a bl)
-          (normal_ret_assert 
-            (EX old:val, 
-              PROPx P (LOCALx (map (subst id (`old)) Q) 
-                (SEPx (`(Post x) (get_result1 id) :: map (subst id (`old)) R))))).
-Proof.
-intros.
-apply semax_call'; auto.
-Qed.
-
-Lemma semax_call0: forall Delta A (Pre Post: A -> assert) (x: A) fsig a bl P Q R,
-   Cop.classify_fun (typeof a) = Cop.fun_case_f (type_of_params (fst fsig)) (snd fsig) ->
-   match fsig with
-   | (_, Tvoid) => True
-   | _ => False
-   end ->
-  semax Delta
-         (PROPx P (LOCALx (tc_expr Delta a :: tc_exprlist Delta (snd (split (fst fsig))) bl :: Q)
-            (SEPx (`(Pre x) ( (make_args' fsig (eval_exprlist (snd (split (fst fsig))) bl))) ::
-                      `(fun_assert_emp fsig A Pre Post) (eval_expr a) :: R))))
-          (Scall None a bl)
-          (normal_ret_assert 
-            (PROPx P (LOCALx Q (SEPx (`(Post x) (make_args nil nil) :: R))))).
-Proof.
-intros.
-eapply semax_pre_post ; [ | | 
-   apply (semax_call Delta A Pre Post x (PROPx P (LOCALx Q (SEPx R))) None fsig a bl H)].
- Focus 3.
- clear - H0.
- destruct fsig. destruct t; simpl in *; try contradiction; split; intros; congruence.
- intro rho; normalize.
-unfold fun_assert_emp.
-repeat rewrite corable_andp_sepcon2 by apply corable_fun_assert.
-normalize.
-rewrite corable_sepcon_andp1 by apply corable_fun_assert.
-rewrite sepcon_comm; auto. 
-intros.
-normalize.
-intro rho; normalize.
-rewrite sepcon_comm; auto.
-Qed.
-
-
-Lemma semax_fun_id':
-      forall id fsig (A : Type) (Pre Post : A -> assert)
-              Delta P Q R PostCond c
-            (GLBL: (var_types Delta) ! id = None),
-            (glob_types Delta) ! id = Some (Global_func (mk_funspec fsig A Pre Post)) ->
-       semax Delta 
-        (PROPx P (LOCALx Q (SEPx (`(fun_assert_emp fsig A Pre Post)
-                         (eval_lvalue (Evar id (type_of_funsig fsig))) :: R))))
-                              c PostCond ->
-       semax Delta (PROPx P (LOCALx Q (SEPx R))) c PostCond.
-Proof.
-intros. 
-apply (semax_fun_id id fsig A Pre Post Delta); auto.
-eapply semax_pre; [ | apply H0].
-forget (eval_lvalue (Evar id (type_of_funsig fsig))) as f.
-intro rho; normalize.
-rewrite andp_comm.
-unfold fun_assert_emp.
-rewrite corable_andp_sepcon2 by apply corable_fun_assert.
-rewrite emp_sepcon; auto.
-Qed.
-
-Lemma eqb_typelist_refl: forall tl, eqb_typelist tl tl = true.
-Proof.
-induction tl; simpl; auto.
-apply andb_true_iff.
-split; auto.
-apply eqb_type_refl.
-Qed.
-
-
-Lemma semax_call_id0:
- forall Delta P Q R id argtys bl fsig A x Pre Post
-   (GLBL: (var_types Delta) ! id = None),
-   (glob_types Delta) ! id = Some (Global_func (mk_funspec fsig A Pre Post)) ->
-   match fsig with
-   | (_, Tvoid) => True
-   | _ => False
-   end ->
-   argtys = type_of_params (fst fsig) ->
-   Tvoid = snd fsig ->
-  semax Delta (PROPx P (LOCALx (tc_exprlist Delta (snd (split (fst fsig))) bl :: Q) (SEPx (`(Pre x) (make_args' fsig (eval_exprlist (snd (split (fst fsig))) bl)) :: R))))
-    (Scall None (Evar id (Tfunction argtys Tvoid)) bl)
-    (normal_ret_assert 
-       (PROPx P (LOCALx Q (SEPx (`(Post x) (make_args nil nil) :: R))))).
-Proof.
-intros.
-assert (Cop.classify_fun (typeof (Evar id (Tfunction argtys Tvoid)))=
-               Cop.fun_case_f (type_of_params (fst fsig)) (snd fsig)).
-rewrite <- H2; subst; reflexivity.
-apply semax_fun_id' with id fsig A Pre Post; auto.
-subst. 
-
-eapply semax_pre; [ | apply (semax_call0 Delta A Pre Post x fsig  _ bl P Q R H3 H0)].
-apply andp_left2.
-apply andp_derives; auto.
-apply andp_derives; auto.
-intro rho; simpl.
-subst.
-autorewrite with normalize.
-apply andp_right.
-apply prop_right. hnf.
-rewrite <- H2 in *.
-simpl.
-unfold get_var_type. rewrite GLBL. rewrite H.
-simpl.
-rewrite eqb_typelist_refl.
-simpl. rewrite <- H2. split; hnf; auto.
-auto.
-change SEPx with SEPx'.
-simpl.
-intro rho.
-rewrite H2.
-rewrite sepcon_comm.
-rewrite sepcon_assoc.
-autorewrite with normalize.
-apply sepcon_derives; auto.
-rewrite sepcon_comm.
-apply sepcon_derives; auto.
-Qed.
-
-Lemma semax_call_id1:
- forall Delta P Q R ret id argtys retty bl fsig A x Pre Post
-   (GLBL: (var_types Delta) ! id = None),
-   (glob_types Delta) ! id = Some (Global_func (mk_funspec fsig A Pre Post)) ->
-   match fsig with
-   | (_, Tvoid) => False
-   | _ => True
-   end ->
-   argtys = type_of_params (fst fsig) ->
-   retty = snd fsig ->
-  semax Delta (PROPx P (LOCALx (tc_exprlist Delta (snd (split (fst fsig))) bl :: Q) (SEPx (`(Pre x) (make_args' fsig (eval_exprlist (snd (split (fst fsig))) bl)) :: R))))
-    (Scall (Some ret)
-             (Evar id (Tfunction argtys retty))
-             bl)
-    (normal_ret_assert 
-       (EX old:val, 
-          PROPx P (LOCALx (map (subst ret (`old)) Q) 
-             (SEPx (`(Post x) (get_result1 ret) :: map (subst ret (`old)) R))))).
-Proof.
-intros.
-assert (Cop.classify_fun (typeof (Evar id (Tfunction argtys retty)))=
-               Cop.fun_case_f (type_of_params (fst fsig)) (snd fsig)).
-subst; reflexivity.
-apply semax_fun_id' with id fsig A Pre Post; auto.
-subst. 
-eapply semax_pre; [ | apply (semax_call1 Delta A Pre Post x ret fsig  _ bl P Q R H3 H0)].
-apply andp_left2.
-apply andp_derives; auto.
-apply andp_derives; auto.
-intro rho; simpl.
-subst.
-autorewrite with normalize.
-apply andp_right.
-apply prop_right. hnf.
-simpl.
-unfold get_var_type. rewrite GLBL. rewrite H.
-simpl.
-rewrite eqb_typelist_refl.
-rewrite eqb_type_refl.
-simpl. split; hnf; auto.
-auto.
-change SEPx with SEPx'.
-simpl.
-intro rho.
-rewrite sepcon_comm.
-rewrite sepcon_assoc.
-autorewrite with normalize.
-apply sepcon_derives; auto.
-rewrite sepcon_comm.
-apply sepcon_derives; auto.
-Qed.
-
-
-Lemma semax_call_id1':
- forall Delta P Q R ret id argtys retty bl fsig A x Pre Post
-   (GLBL: (var_types Delta) ! id = None),
-   (glob_types Delta) ! id = Some (Global_func (mk_funspec fsig A Pre Post)) ->
-   match fsig with
-   | (_, Tvoid) => False
-   | _ => True
-   end ->
-   argtys = type_of_params (fst fsig) ->
-   retty = snd fsig ->
-  forall 
-   (CLOSQ: Forall (closed_wrt_vars (eq ret)) Q)
-   (CLOSR: Forall (closed_wrt_vars (eq ret)) R),
-  semax Delta (PROPx P (LOCALx (tc_exprlist Delta (snd (split (fst fsig))) bl :: Q) (SEPx (`(Pre x) (make_args' fsig (eval_exprlist (snd (split (fst fsig))) bl)) :: R))))
-    (Scall (Some ret)
-             (Evar id (Tfunction argtys retty))
-             bl)
-    (normal_ret_assert 
-       (PROPx P (LOCALx Q   (SEPx (`(Post x) (get_result1 ret) ::  R))))).
-Proof.
-intros.
-eapply semax_post;
-  [ | apply (semax_call_id1 Delta P Q R ret id argtys retty bl fsig A x Pre Post 
-     GLBL H H0 H1 H2)].
-intros ek vl.
-apply andp_left2.
-unfold normal_ret_assert.
-apply andp_derives; auto.
-apply andp_derives; auto.
-apply exp_left; intro v.
-apply andp_derives; auto.
-apply andp_derives.
-unfold local, lift1 ;intro rho.
-clear - CLOSQ.
-apply prop_left. intro.
-apply prop_right.
-induction Q; simpl; auto.
-inv CLOSQ.
-destruct H.
-split.
-rewrite closed_wrt_subst in H; auto.
-auto.
-clear - CLOSR.
-change SEPx with SEPx'.
-unfold SEPx'. intro rho.
-simpl.
-apply sepcon_derives; auto.
-induction R; simpl; auto.
-inv CLOSR.
-apply sepcon_derives.
-rewrite closed_wrt_subst; auto.
-apply IHR; auto.
-Qed.
-
-Lemma semax_call_id1_Eaddrof:
- forall Delta P Q R ret id argtys retty bl fsig A x Pre Post
-   (GLBL: (var_types Delta) ! id = None),
-   (glob_types Delta) ! id = Some (Global_func (mk_funspec fsig A Pre Post)) ->
-   match fsig with
-   | (_, Tvoid) => False
-   | _ => True
-   end ->
-   argtys = type_of_params (fst fsig) ->
-   retty = snd fsig ->
-  semax Delta (PROPx P (LOCALx (tc_exprlist Delta (snd (split (fst fsig))) bl :: Q) (SEPx (`(Pre x) (make_args' fsig (eval_exprlist (snd (split (fst fsig))) bl)) :: R))))
-    (Scall (Some ret)
-             (Eaddrof (Evar id (Tfunction argtys retty)) (Tpointer (Tfunction argtys retty) noattr))
-             bl)
-    (normal_ret_assert 
-       (EX old:val, 
-          PROPx P (LOCALx (map (subst ret (`old)) Q) 
-             (SEPx (`(Post x) (get_result1 ret) :: map (subst ret (`old)) R))))).
-Proof.
-intros.
-assert (Cop.classify_fun (typeof (Eaddrof (Evar id (Tfunction argtys retty)) (Tpointer (Tfunction argtys retty) noattr)))=
-               Cop.fun_case_f (type_of_params (fst fsig)) (snd fsig)).
-subst; reflexivity.
-apply semax_fun_id' with id fsig A Pre Post; auto.
-subst. 
-eapply semax_pre; [ | apply (semax_call1 Delta A Pre Post x ret fsig  _ bl P Q R H3 H0)].
-apply andp_left2.
-apply andp_derives; auto.
-apply andp_derives; auto.
-intro rho; simpl.
-subst.
-autorewrite with normalize.
-apply andp_right.
-apply prop_right. hnf.
-simpl.
-unfold get_var_type. rewrite GLBL. rewrite H.
-simpl.
-rewrite eqb_typelist_refl.
-rewrite eqb_type_refl.
-simpl. apply I.
-auto.
-change SEPx with SEPx'.
-simpl.
-intro rho.
-cancel.
-Qed.
-
-
-Lemma semax_call_id_aux1: forall P Q1 Q R S,
-     PROPx P (LOCALx (Q1::Q) R) |-- S -> local Q1 && PROPx P (LOCALx Q R) |-- S.
-Proof. intros. eapply derives_trans; try apply H.
-  intro rho; normalize.
- unfold PROPx. simpl.
- apply andp_derives; auto.
- unfold LOCALx. simpl.
- unfold local,lift2,lift1.
- apply derives_extract_prop; intro.
- apply andp_right; auto.
- apply prop_right; split; auto.
-Qed.
-
-(* BEGIN HORRIBLE1.
-  The following lemma is needed because CompCert clightgen
- produces the following AST for function call:
-  (Ssequence (Scall (Some id') ... ) (Sset id (Etempvar id' _)))
-instead of the more natural
-   (Scall id ...)
-Our general tactics are powerful enough to reason about the sequence,
-one statement at a time, but it is not nice to burden the user with knowing
-about id'.  So we handle it all in one gulp.
- See also BEGIN HORRIBLE1 in forward.v
-*)
-
-
-Lemma semax_call_id1_x:
- forall Delta P Q R ret ret' id argtys retty bl fsig A x Pre Post
-   (GLBL: (var_types Delta) ! id = None),
-   (glob_types Delta) ! id = Some (Global_func (mk_funspec fsig A Pre Post)) ->
-   match fsig with
-   | (_, Tvoid) => False
-   | _ => True
-   end ->
-   argtys = type_of_params (fst fsig) ->
-   retty = snd fsig ->
-  forall
-   (CLOSQ: Forall (closed_wrt_vars (eq ret')) Q)
-   (CLOSR: Forall (closed_wrt_vars (eq ret')) R),
-   type_is_volatile retty = false -> 
-   (temp_types Delta) ! ret' = Some (retty, false) ->
-   is_neutral_cast retty retty = true ->
-   match (temp_types Delta) ! ret with Some (t,_) => eqb_type t retty | None => false end = true ->
-  semax Delta (PROPx P (LOCALx (tc_exprlist Delta (snd (split (fst fsig))) bl :: Q) (SEPx (`(Pre x) (make_args' fsig (eval_exprlist (snd (split (fst fsig))) bl)) :: R))))
-    (Ssequence (Scall (Some ret')
-             (Evar id (Tfunction argtys retty))
-             bl)
-      (Sset ret (Etempvar ret' retty)))
-    (normal_ret_assert 
-       (EX old:val, 
-          PROPx P (LOCALx (map (subst ret (`old)) Q) 
-             (SEPx (`(Post x) (get_result1 ret) :: map (subst ret (`old)) R))))).
-Proof.
- intros. rename H3 into NONVOL.
- eapply semax_seq'.
- apply (semax_call_id1' _ P Q R ret' _ _ _ bl _ _ x _ _ GLBL H H0 H1 H2 CLOSQ CLOSR).
-match goal with |- semax ?D (PROPx ?P ?QR) ?c ?Post =>
-   assert ( (fold_right and True P) -> semax D (PROPx nil QR) c Post)
- end.
-Focus 2.
- clear - H3.
- unfold PROPx. 
- unfold PROPx at 1 in H3.
- normalize in H3.
- apply semax_extract_prop. apply H3.
- (* End Focus 2 *)
- intro.
- apply semax_post_flipped
- with (normal_ret_assert (EX  x0 : val,
-PROP  ()
-(LOCALx
-   (tc_environ
-      (initialized ret
-         (update_tycon Delta
-            (Scall (Some ret') (Evar id (Tfunction argtys retty)) bl)))
-    :: `eq (eval_id ret)
-         (subst ret (`x0) (eval_expr (Etempvar ret' retty)))
-       :: map (subst ret (`x0)) Q)
-   (SEPx
-      (map (subst ret (`x0)) (`(Post x) (get_result1 ret') :: R)))))).
-  make_sequential;
-          eapply semax_post_flipped;
-          [ apply forward_setx; 
-            try solve [intro rho; rewrite andp_unfold; apply andp_right; apply prop_right;
-                            repeat split ]
-           | intros ?ek ?vl; apply after_set_special1 ].
- apply andp_right.
- intro rho; unfold tc_expr; simpl.
- rewrite NONVOL. simpl.
- replace ( (temp_types (initialized ret' Delta)) ! ret' ) 
-     with (Some (retty, true)).
-Focus 2.
- unfold initialized;  simpl. rewrite H4.
- unfold temp_types; simpl.
- rewrite PTree.gss. auto.
- (* End Focus 2 *)
- unfold local; apply prop_right.
- simpl. rewrite eqb_type_refl. apply I.
- intro rho; apply prop_right; unfold tc_temp_id; simpl.
- unfold typecheck_temp_id.
- destruct (eq_dec ret' ret).
- subst ret'.
- unfold temp_types. unfold initialized; simpl.
- rewrite H4. simpl. rewrite PTree.gss.
- rewrite H5.
- simpl.
- unfold isCastResultType. unfold is_neutral_cast in H5.
- destruct (Cop.classify_cast retty retty); try discriminate.
- rewrite eqb_type_refl. apply I.
- unfold temp_types. unfold initialized; simpl.
- rewrite H4. simpl. rewrite PTree.gso by auto. 
- destruct ((temp_types Delta) ! ret); try discriminate.
- destruct p. apply eqb_type_true in H6.
- subst t. rewrite H5.
- simpl.
- unfold isCastResultType. unfold is_neutral_cast in H5.
- destruct (Cop.classify_cast retty retty); try discriminate.
- rewrite eqb_type_refl. apply I.
- auto.
- intros.
- apply andp_left2. apply normal_ret_assert_derives'.
- apply exp_derives; intro old.
- apply andp_derives.
- apply prop_right; auto.
- intro rho; unfold LOCALx, local.
-change SEPx with SEPx'.
- simpl. 
-  normalize.
- unfold coerce, lift1_C, lift0_C.
- apply sepcon_derives; auto.
- normalize.
- replace (subst ret (lift0 old) (get_result1 ret') rho)
-   with (get_result1 ret rho); auto.
- destruct (eq_dec ret ret').
- subst.
- unfold get_result1.
- unfold subst. f_equal.
- normalize in H8.
- normalize. f_equal. auto.
- clear - H6 H8 H7.
- unfold tc_environ in H7.
- unfold env_set. destruct rho; simpl in *; f_equal.
- unfold eval_id in H8; simpl in H8. unfold subst in H8.
- simpl in *. rewrite Map.gss in H8. simpl in H8.
- unfold_coerce. subst.
- unfold Map.set. extensionality i. 
- destruct (ident_eq i ret'); auto.  subst i.
- unfold typecheck_environ in H7.
- repeat rewrite andb_true_iff in H7.
- destruct H7 as [[[? _] _] _].
- simpl te_of in H.
- apply environ_lemmas.typecheck_te_eqv in H.
- hnf in H.
- specialize (H ret').
- revert H6; case_eq ((temp_types Delta)!ret'); intros; try discriminate.
- destruct p.
- unfold temp_types, initialized in H; simpl in H.
- rewrite H0 in H. unfold temp_types in *. simpl in H. rewrite PTree.gss in H.
- simpl in H. rewrite PTree.gss in H.
- specialize (H true t (eq_refl _)). 
- destruct H as [v [? ?]]. rewrite H.
- apply H.
-  rewrite closed_wrt_subst; auto with closed.
- unfold get_result1.
- f_equal. f_equal.
- rewrite H8.
-  rewrite closed_wrt_subst; auto with closed.
-Qed.
-
-(* END HORRIBLE1 *)
-
